\textbf{Extra Credit}

Prove that $\lim\limits_{n \to \infty} {a_n} = 0$, where $a_n = \left(\frac{1}{n!}\right)^{\frac{1}{n}}$.

\begin{solution}
    We first observe that each $a_n$ is strictly positive, and hence $\lim\limits_{n \to \infty} {a_n} \ge 0$.
    Moreover, for any particular $n, j \in \mathbb{N}$ with $1 \le j \le \frac{n}{2}$, we have

    $$
    (n - j + 1) j \ge (n - 1 + 1) j = n j \ge n.
    $$

    Without loss of generality, we suppose that $n$ is even (if it is not, we simply replace $n$ with $n + 1$ and all 
    calculations remain the same). Then we have:

    $$
        \frac{1}{n!} = \frac{1}{n \cdot (n - 1) \cdots 2 \cdot 1} 
                     = \frac{1}{\prod_{j=0}^{n/2}(n - j + 1) j}
                     \le \frac{1}{\prod_{j=0}^{n/2} n}
                     = \frac{1}{n^{\frac{n}{2}}}
    $$ 

    so that

    $$
    0 \le a_n = \left(\frac{1}{n!}\right)^{\frac{1}{n}} 
              \le \left(\frac{1}{n^{\frac{n}{2}}}\right)^{\frac{1}{n}}
              = \sqrt{\frac{1}{n}}
    $$

    and hence $\lim\limits_{n \to \infty} {a_n} = 0$ by the squeeze theorem.
\end{solution}