\textbf{Stein, Shakarchi 1.2}

Let $\langle \cdot, \cdot \rangle$ denote the usual inner product on $\mathbb{R}^2$ and $(z, w) = z \bar{w}$ a Hermitian 
inner product on $\mathbb{C}$. Show that 

$$
\langle z, w \rangle = \frac{1}{2} \left[ (z, w) + (w, z) \right] = \text{Re}(z, w)
$$

\begin{solution}
    Let $z = x + iy$ and $w = u + iv$, where $x, y, u, v \in \mathbb{R}$. Then we have

    $$
    (z, w) = (x + iy)\overline{(u + iv)} = (x + iy)(u - iv) = xu + yv + i(yu - xv)
    $$

    and hence $\text{Re}(z, w) = xu + yv = \langle z, w \rangle$. Moreover, we have

    $$
    (w, z) = \overline{(z, w)} = \overline{xu + yv + i(yu - xv)} = xu + yv - i(yu - xv) 
    $$

    so that upon adding $(z, w)$ and $(w, z)$, the terms $i(yu - xv)$ and $-i(yu - xv)$ cancel and we are left with

    \begin{align*}
        \frac{1}{2} \left[ (z, w) + (w, z) \right] = \frac{1}{2} (2xu + 2yv) = xu + yv = \langle z, w \rangle
    \end{align*}

    as desired.
    \ \\
\end{solution}
