Prove that the solution to this problem is given by

$$
x_* = r + \frac{b - a^T r}{a^T a} a.
$$

\begin{solution}
    We begin by constructing the Lagrangian for this problem, which is given by

    $$
    \mathcal{L}(x, \lambda) = f(x) - \lambda g(x) = \frac{1}{2} (x - r)^T I (x - r) - \lambda (a^T x - b)
    $$

    where $\lambda$ is a scalar since our system only contains a single constraint. We note that the Lagrangian is a 
    quadratic form where $I$ is symmetric and positive definite. We compute corresponding stationary points by setting 
    the gradient of the Lagrangian (with respect to $x$) to zero, which yields

    $$
    \nabla_x \mathcal{L} = (x - r) - \lambda a = 0
    $$

    so that $x_* = r + \lambda a$. We substitute this expression into our equality constraint to find

    $$
    b = a^T x_* = a^T (r + \lambda) a = a^T r + \lambda a^T a
    $$

    to find that $\lambda = \frac{b - a^T r}{a^T a}$ (where we have used the fact that $a^T a$ is a scalar value). Our 
    stationary point is thus

    $$
    x_* = r + \lambda a = r + \frac{b - a^T r}{a^T a} a
    $$

    as desired. Finally, since our Lagrangian is a quadratic form with positive definite matrix $I$, we know that $x_*$
    is the unique global minimizer of $f$.
    \ \\
\end{solution}