Solve the linear program with the result from (b).

\begin{solution}

    We use our result from (a) as our initial basis to solve the original program so that $x_B = \{ x_1 \}$ and 
    $x_N = \{ x_2, x_3 \}$ (where we have dropped the artificial variable from the problem now that we have obtained a
    basic feasible solution to start the simplex method with). At the first iteration, our simplex quantities of interest are given by

    \begin{align*}
      B &= \begin{pmatrix}
        1  \\
      \end{pmatrix}, \quad y = \begin{pmatrix}
        1 
      \end{pmatrix}^T, \quad c_B = \begin{pmatrix}
        1
      \end{pmatrix}^T \\
      \hat{b} &= \begin{pmatrix}
        2
      \end{pmatrix}^T, \quad \hat{c}_N = \begin{pmatrix}
        -2 & -1 
      \end{pmatrix}^T, \quad \tilde{z} = 2.
    \end{align*}

    We choose $x_2$ as our entering variable and $x_1$ to leave the basis (since it is the only one in the basis),
    which yields

    \begin{align*}
      B &= \begin{pmatrix}
        1  \\
      \end{pmatrix}, \quad y = \begin{pmatrix}
       -1 
      \end{pmatrix}^T, \quad c_B = \begin{pmatrix}
       -1
      \end{pmatrix}^T \\
      \hat{b} &= \begin{pmatrix}
        2
      \end{pmatrix}^T, \quad \hat{c}_N = \begin{pmatrix}
        1 & 1
      \end{pmatrix}^T, \quad \tilde{z} = -2.
    \end{align*}

    Since all elements of the reduced cost vector are nonnegative, we have found an optimal solution to the original
    program which occurs at the point $(x_1', x_2', x_3') = (0, 2, 0)$ with objective value $\tilde{z} = -2$. We apply
    the inverse of our original affine transformations of $x_1$ and $x_2$ to find that the optimal solution to the 
    original program is given by $(x_1, x_2) = (3, 3)$ with objective value $z = 6$.

\end{solution}