\textbf{Stein, Shakarchi 2.4}

Prove that for all $\xi \in \mathbb{C}$, we have

$$
e^{-\pi \xi^2} = \int_{-\infty}^{\infty} {e^{-\pi x^2} e^{2 \pi i x \xi} \; dx}.
$$

\begin{solution}
    Let $\xi = a + bi$, where $a, b \in \mathbb{R}$. Completing the square for $x^2 - 2 i x \xi$ yields

    $$
    x^2 - 2 i x \xi = (x - i\xi)^2 + \xi^2
    $$

    so that we have

    \begin{align*}
        \int_{-\infty}^{\infty} {e^{-\pi x^2} e^{2 \pi i x \xi} \; dx} &= \int_{-\infty}^{\infty} {e^{-\pi (x^2 - 2 i x \xi)} \; dx} \\
                                                                       &= \int_{-\infty}^{\infty} {e^{-\pi \left( (x - i\xi)^2 + \xi^2 \right)} \; dx} \\
                                                                       &= e^{-\pi \xi^2}\int_{-\infty}^{\infty} {e^{-\pi \left( x - i(a + bi)\right)^2} \; dx} \\
                                                                       &= e^{-\pi \xi^2}\int_{-\infty}^{\infty} {e^{-\pi \left((x + b) - ai \right)^2} \; dx}.
    \end{align*}

    Letting $u = x + b$, we have $du = dx$ so that

    \begin{align*}
        e^{-\pi \xi^2}\int_{-\infty}^{\infty} {e^{-\pi \left((x + b) - ai \right)^2 } \; dx} 
          &=e^{-\pi \xi^2}\int_{-\infty}^{\infty} {e^{-\pi \left(u^2 - 2 i u a - a^2 \right)} \; du} \\
          &=e^{-\pi \xi^2} e^{\pi a^2} \int_{-\infty}^{\infty} {e^{-\pi u^2} e^{2 \pi i u a } \; du} \\
          &=e^{-\pi \xi^2} e^{\pi a^2} e^{-\pi (-a)^2} \\
          &=e^{-\pi \xi^2} 
    \end{align*}

    where we have used the fact that for \textit{real} $a, x \in \mathbb{R}$, we have

    $$
    e^{-\pi a^2} = \int_{-\infty}^{\infty} e^{-\pi x^2} e^{-2 \pi i x a}\; dx.
    $$

    \ \\
\end{solution}