Prove that for $\lambda \in \mathbb{R} \setminus \{0, 1\}$, the function

$$
f(z) = \int_0^z \frac{d\zeta}{\sqrt{\zeta (\zeta - 1)(\zeta - \lambda)}}
$$

is a conformal map from the upper half-plane $\mathbb{H}$ to a rectangle such that one of the rectangle's vertices is 
the image of the point at infinity.

\begin{solution} 
  Without loss of generality, we suppose that $\lambda > 1$, as changing where $\lambda$ lies on the real axis merely 
  changes the order of the resulting vertices. We also choose an appropriate branch of the denominator of $f$ so that 
  the denominator is positive whenever $\zeta$ is real and $0 < \zeta < \lambda$. Let $A_1 = 0$, $A_2 = 1$, and 
  $A_3 = \lambda$ and let $\beta_1 = \beta_2 = \beta_3 = \frac{1}{2}$. We begin by observing that 

  $$
  \beta_j < 1 \quad \text{and} \quad 1 < \sum_{k=1}^{3} \beta_k = \frac{3}{2} < 2,
  $$

  so that by Proposition 4.1, the image of the real axis under $f$ is a polygon of four sides with vertices 
  $a_1, a_2, a_3$, and $a_{\infty}$ where $f(A_j) = a_j$, $f(\infty) = a_{\infty}$, and the angle at the vertex 
  $a_{\infty}$ is given by 
  
  $$
    \left[1 - \left(2 - \sum\limits_{k = 1}^3 \beta_k \right) \right] = \frac{\pi}{2}.
  $$

  Furthermore, the interior angles at $a_j$ are given by $\pi (1 - \beta_j) = \frac{\pi}{2}$, so that the image of the 
  real line under $f$ is a rectangle $R$ with vertices $a_1 = f(0) = 0$, $a_2 = f(1)$, $a_3 = f(\lambda)$, and 
  $a_{\infty} = f(\infty)$. It remains to show that $f$ is a conformal map from $\mathbb{H}$ to $R$. By Theorems 4.6 and 
  4.7, we know that there exist complex numbers $C_1 \neq 0$ and $C_2$ such that the conformal map $F$ of $\mathbb{H}$ 
  to $R$ is given by

  $$
  F(z) = C_1 \int_0^z \frac{d\zeta}{\sqrt{\zeta(\zeta - 1)(\zeta - \lambda)}} + C_2.
  $$

  Moreover, $f(A_1) = f(0)$ is given by

  $$
  f(A_1) = f(0) = \int_0^0 \frac{d\zeta}{\sqrt{\zeta(\zeta - 1)(\zeta - \lambda)}} = 0 = a_1,
  $$

  and since $F$ also maps $A_1$ to $a_1$, we conclude that $F(0) = 0$ so that $C_2 = 0$. Similarly, since 
  $f(A_2) = f(1) = a_2$ and noting that $F(1)$ must equal $a_2$, we have

  $$
  F(1) = C_1 \int_0^1 \frac{d\zeta}{\sqrt{\zeta(\zeta - 1)(\zeta - \lambda)}} = a_2 = f(1) = \int_0^1 \frac{d\zeta}{\sqrt{\zeta(\zeta - 1)(\zeta - \lambda)}},  
  $$

  so that $C_1 = 1$ and $F(z) = f(z)$ for all $z \in \mathbb{H}$, which shows that $f(z) = F(z)$ is a conformal map
  from $\mathbb{H}$ to $R$.
  \ \\
\end{solution}