What would the new solution be if the coefficient of $x_1$ in the objective were decreased by 2? Increased by 2?

\begin{solution}
  Recall from Example 6.14 that

  $$
  B^{-1} N = \begin{pmatrix*}[r]
     \sfrac{1}{2} & \sfrac{1}{2} \\
                0 &            1 \\
    -\sfrac{1}{2} & \sfrac{3}{2}
  \end{pmatrix*}, \quad c_B = \begin{pmatrix*}
    -2 \\
    -1 \\
     0
  \end{pmatrix*}
  $$

  Let $\delta$ be the change in the coefficient of $x_1$ in the objective so that $\bar{c}_B = c_B + \Delta c$ where 
  $\Delta c = (0, \delta, 0)^T$.\footnote{
    Recall that our current basis is $x_B = (x_2, x_1, x_2)^T$ and so the second element of $\Delta c$ represents a 
    change in the coefficient of $x_1$.
  } The current basis remains optimal so long as \linebreak
  $c_N^T - \bar{c}_B^T B^{-1} N \ge 0 $. Hence we impose the condition

  \begin{align*}
    c_N^T - \bar{c}_B^T B^{-1} N &= (0, 0)^T - (c_B + \Delta c_B) B^{-1} N \\
                                 &= -c_B^T B^{-1} N - \Delta c_B^T B^{-1} N \\
                                 &= (2, 1, 0) \begin{pmatrix*}[r]
                                        \sfrac{1}{2} & \sfrac{1}{2} \\
                                                   0 &            1 \\
                                       -\sfrac{1}{2} & \sfrac{3}{2}
                                    \end{pmatrix*} + (0, \delta, 0) \begin{pmatrix*}[r]
                                        \sfrac{1}{2} & \sfrac{1}{2} \\
                                                   0 &            1 \\
                                       -\sfrac{1}{2} & \sfrac{3}{2}
                                    \end{pmatrix*} \\
                                 &= \begin{pmatrix*}
                                      1 \\
                                      2 + \delta
                                    \end{pmatrix*} \\
                                 &\ge 0.
  \end{align*}

  The current basis is therefore optimal so long as $\delta \ge -2$. For any particular $\delta$, the new solution 
  $\bar{z}$ is given by

  \begin{align*}
  \bar{z} &= \bar{c}_B^T B^{-1} b \\
          &= \left(c_B^T + \Delta c_B^T \right) B^{-1} b \\
          &= y^T b + \Delta c_B^T B^{-1} b \\
          &= (0, -1, -2)(2, 7,  3)^T + (0, \delta, 0)(5, 3, 3)^T \\
          &= -13 + 3\delta.
  \end{align*}

  Increasing the coefficient of $x_1$ in the objective function (i.e., letting $\delta = 2$) yields 
  $\bar{z}^+ = -13 + 6 = -7$, and decreasing the coefficient by two ($\delta = -2$) yields $\bar{z}^- = -13 - 6 = -19$.
  \footnote{
    The resulting values for $x_B$ are computed in \texttt{problem\_9iii\_increase.py} and 
    \texttt{problem\_9iii\_decrease.py} for the interested reader.
  }
  \ \\
  \vfill
\end{solution}
