\textbf{Stein, Shakarchi 3.7}

Prove that 

$$
\int_0^{2 \pi} {\frac{d \theta}{(a + \cos{\theta})^2}} = \frac{2 \pi a}{(a^2 - 1)^{3/2}}, \quad a > 1.
$$

\begin{solution}
  Let $z_{a^+} = -a + \sqrt{a^2 - 1}$ and $z_{a^-} = -a - \sqrt{a^2 - 1}$, and let

  $$
  f(z) = \frac{4 z}{(z - z_{a^+})^2 (z - z_{a^-})^2}.
  $$
  
  With the parametrization $z = e^{i \theta}$, we find

  \begin{align*}
    \int_{|z| = 1} { f(z) \; dz } 
      &= \int_{|z| = 1} { \frac{4 z}{(z - z_{a^+})^2 (z - z_{a^-})^2} \; dz } \\
      &= \int_{|z| = 1} { \frac{1}{z} \left( \frac{2z}{z^2 + 2 a z + 1} \right)^2 \; dz } \\
      &= \int_0^{2 \pi} { e^{-i \theta} \left( \frac{2}{e^{i \theta} + 2 a + e^{-i \theta}} \right)^2 i e^{i \theta} \; d\theta } \\
      &= i \int_0^{2 \pi} {\frac{1}{(a + \cos{\theta})^2} \; d\theta } \\
  \end{align*}

  We apply the residue theorem to $f(z)$ over the unit disc. We note that while $z_{a^+}$ and $z_{a^-}$ are both poles 
  of $f(z)$ each of order two, only $z_{a^+}$ lies inside the unit disc. Hence we find

  \begin{align*}
    \int_{|z| = 1} { f(z) \; dz } 
      &= 2 \pi i \lim_{z \to z_{a^+}} \frac{d}{dz} \left[ (z - z_{a^+})^2 \frac{4z}{(z - z_{a^+})^2 (z - z_{z_a^-})^2} \right] \\
      &= 2 \pi i \lim_{z \to z_{a^+}} \frac{d}{dz} \left[ \frac{4z}{(z - z_{z_a^-})^2} \right] \\
      &= 8 \pi i \lim_{z \to z_{a^+}} \frac{(z - z_{a^-})^2 - 2 z (z - z_{a^-})}{(z - z_{z_a^-})^4} \\
      &= 8 \pi i \lim_{z \to z_{a^+}} \frac{(z - z_{a^-}) - 2 z }{(z - z_{z_a^-})^3} \\
      &= 8 \pi i \cdot \frac{2\sqrt{a^2 - 1} - 2(-a + \sqrt{a^2 - 1})}{(2\sqrt{a^2 - 1})^3} \\
      &= i \frac{2 \pi a}{(a^2 - 1)^{3/2}}
  \end{align*}

  \pagebreak
  where we have used the fact that

  $$
  z_{a^+} - z_{a^-} = 2 \sqrt{a^2 - 1}.
  $$

  Hence we have 

  $$
    i \int_0^{2 \pi} {\frac{1}{(a + \cos{\theta})^2} \; d\theta } = \int_{|z| = 1} {f(z) \; dz} 
                                                                  = i \frac{2 \pi a}{(a^2 - 1)^{3/2}}
  $$
  so that 

  $$
    \int_0^{2 \pi} {\frac{1}{(a + \cos{\theta})^2} \; d\theta } = \frac{2 \pi a}{(a^2 - 1)^{3/2}}
  $$

  as desired.

  \ \\
\end{solution}