\textbf{Stein, Shakarchi 3.6}

Show that for $n \ge 1$, we have

$$
  \int_{-\infty}^{\infty} {\frac{dx}{\left( 1 + x^2 \right)^{n+1}}} = \pi \cdot \frac{\prod\limits_{k=1}^{n} (2k - 1)}{\prod\limits_{k=1}^{n} (2k)}
$$

\begin{solution}
  We fix $n \in \mathbb{N}$ and observe that poles exist at $z = i$ and $z = -i$, each of order $n + 1$. Integrating 
  over the semicircle $\gamma_R$ of radius $R > 1$ (so that $z = i$ is contained in the closed curve) and applying the 
  residue theorem yields:

  \begin{align*}
    \int_{\gamma_R} { \frac{1}{(1 + z^2)^{n+1}} \; dz } 
      &= \lim\limits_{z \to i} \frac{1}{n!} \left(\frac{d}{dz}\right)^n (z - i)^{n+1} \frac{1}{(1 + z^2)^{n+1}} \\
      &= \lim\limits_{z \to i} \frac{1}{n!} \left(\frac{d}{dz}\right)^n \frac{1}{(z + i)^{n+1}} \\
      &= \lim\limits_{z \to i} \frac{1}{n!} \left(\frac{d}{dz}\right)^{n-1} \frac{-(n+1)}{(z + i)^{n+2}} \\
      &\vdots \\
      &= \lim\limits_{z \to i} \frac{1}{n!} \frac{(2n)!}{n!} \frac{(-1)^n}{(z + i)^{2n}} \\
      &= \frac{(2n)!}{n! \, n! \, 2^{2n}} \\
      &= \frac{1 \cdot 2 \cdots (2n)}{n! \, n! \, 2^{2n}} \\
      &= \frac{[1 \cdot 3 \cdots (2n - 1)] \cdot 2 \cdot 4 \cdots 2n}{n! \, n! \, 2^{2n}} \\
      &= \frac{[1 \cdot 3 \cdots (2n - 1)] 2^n \, n!}{n! \, n! \, 2^{2n}} \\
      &= \frac{[1 \cdot 3 \cdots (2n - 1)]}{n! \, 2^n} \\
      &= \frac{1 \cdot 3 \cdots (2n - 1)}{2 \cdot 4 \cdots 2n}.
  \end{align*}

  To obtain the desired result, we observe that together with the parametrization of 
  $z = e^{i \theta}$ for $\theta \in [0, \pi]$, the integral over the semicircle $\gamma_R$ is given by

  $$
    \int_{\gamma_R} { \frac{1}{(1 + z^2)^{n+1}} \; dz } = \int_{-R}^{R} { \frac{1}{(1 + x^2)^{n+1}} \; dx } 
                                                        + \int_0^{\pi} { \frac{i R e^{i \theta}}{\left(1 + R^2 e^{2 i \theta}\right)^{n+1}} \; d\theta }
  $$

  \pagebreak
  We bound the latter integral as before via the reverse triangle inequality to obtain:

  \begin{align*}
    \left|\int_0^{\pi} { \frac{i R e^{i \theta}}{\left(1 + R^2 e^{2 i \theta}\right)^{n+1}} \; d\theta } \right|
      &\le \int_0^{\pi} { \frac{R}{\left| 1 + R^2 e^{2 i \theta} \right|^{n+1}} \; d\theta} \\
      &\le \int_0^{\pi} { \frac{R}{\left| 1 - R^2 \right|^{n+1}} \; |d\theta|} \\
      &= \frac{2 \pi R^2}{\left| 1 - R^2 \right|^{n+1}}
  \end{align*}

  which tends to zero as $R \to \infty$ whenever $n \ge 1$. We combine this result with the above residue calculation to 
  obtain in the limit that 

  $$
    \int_{-\infty}^{\infty} { \frac{1}{(1 + x^2)^{n+1}} \; dx } 
      = \int_{\gamma_{\infty}} { \frac{1}{(1 + z^2)^{n+1}} \; dz } 
      = \frac{1 \cdot 3 \cdots (2n - 1)}{2 \cdot 4 \cdots 2n}
  $$ 

  as desired.

  \ \\
\end{solution}