Given $\alpha \in \mathbb{D}$, find real numbers $a, b, c, d$ such that $ad - bc = 1$ and so that for any 
$z \in \mathbb{H}$, the following holds:

$$
\frac{az + b}{cz + d} = f^{-1} \left(\psi_{\alpha} (f(z)) \right),
$$

where $\psi_{\alpha}(z) = \frac{\alpha - z}{1 - \conj{\alpha}z}$ (where in general, $\alpha \in \mathbb{C}$ and $|\alpha| < 1$).

\begin{solution}
  We proceed as in (a), letting $M_{\psi_{\alpha}}$ denote the matrix of the linear transformation $\psi_{\alpha}(z)$
  which is given by

  $$
  M_{\psi_\alpha} = \begin{pmatrix}
    -1            & \alpha \\
    -\conj{\alpha} & 1
  \end{pmatrix}
  $$

  Our desired transformation is given by:


  \begin{align*}
    M_{f^{-1}} M_{\psi_\alpha} M_f &= \begin{pmatrix}
      -i & i \\
       1 & 1
    \end{pmatrix} \begin{pmatrix}
      -1             & \alpha \\
      -\conj{\alpha} & 1
    \end{pmatrix} \begin{pmatrix}
      -1 & i \\
       1 & i
    \end{pmatrix} \\
    &= \begin{pmatrix}
      -i & i \\
       1 & 1
    \end{pmatrix} \begin{pmatrix}
      1 + \alpha        & i(\alpha -1) \\
      \conj{\alpha} + 1 & i(1 - \conj{\alpha})
    \end{pmatrix} \\
    &= \begin{pmatrix}
      i(\conj{\alpha} - \alpha)  & \alpha + \conj{\alpha} - 2 \\
      \alpha + \conj{\alpha} + 2 & i(\alpha - \conj{\alpha})
    \end{pmatrix} \\
    &= 2 \begin{pmatrix}
      \text{Im}(\alpha)     &  \text{Re}(\alpha) - 1 \\
      \text{Re}(\alpha) + 1 & -\text{Im}(\alpha)
    \end{pmatrix}.
  \end{align*}

  We note that the determinant of this matrix is given by 
  $-\text{Im}^2(\alpha) - \text{Re}^2(\alpha) + 1 = 1 - |\alpha|^2$. We define
  $K = \left(1 - |\alpha|^2\right)^{-\frac{1}{2}}$ and let $a = K \text{Im}(\alpha)$, $b = K(\text{Re}(\alpha) - 1)$,
  $c = K(\text{Re}(\alpha) + 1)$, and $d = -K \text{Im}(\alpha)$; under these definitions, we obtain the following 
  fractional linear transformation determined by the above matrix:

  $$
  \Phi_b = \frac{2 \text{Im}(\alpha)z + 2(\text{Re}(\alpha) - 1)}{2(\text{Re}(\alpha) + 1)z - 2\text{Im}(\alpha)}
         = \frac{K \text{Im}(\alpha)z + K(\text{Re}(\alpha) - 1)}{K(\text{Re}(\alpha) + 1)z - K\text{Im}(\alpha)}
         = \frac{az + b}{cz + d}
  $$

  where $ad - bc = 1$ by construction. We therefore conclude that $a, b, c,$ and $d$ are the desired real numbers and 
  define

  $$
  M_{\Phi_b} = \begin{pmatrix}
    a & b \\
    c & d
  \end{pmatrix} = \begin{pmatrix}
    K \text{Im}(\alpha) & K(\text{Re}(\alpha) - 1) \\
    K(\text{Re}(\alpha) + 1) & -K \text{Im}(\alpha)
  \end{pmatrix}.
  $$
  \ \\
\end{solution}