a.  Let $\{a_k\}$ be a real sequence. Define
    $\sigma_n \coloneqq \frac{a_1 + a_2 + \cdots + a_n}{n}$. If 
    $\lim_{k \rightarrow \infty}{a_k} = a$, prove that
     $\lim_{n \rightarrow \infty}{\sigma_n} = a$.  Show that the converse is
    false.

    \begin{proof}\ \\\\

        Observe that since $\lim_{k \rightarrow \infty}{a_k} = a$, there exists
        for each fixed $\epsilon > 0$ some $N \in \mathbb{N}$ such that
        whenever $k > N$, $|a_k - a| < \frac{\epsilon}{2}$. Then for
        $n > N$, we have:

        \begin{align*}
            |\sigma_n - a|
             &= \left|\frac{1}{n}\sum\limits_{k=1}^{n}{a_k} - \frac{1}{n}\sum\limits_{k=1}^{n}{a} \right| \\
             &= \left|\frac{1}{n}\sum\limits_{k=1}^{n}{\left(a_k - a\right)} \right| \\
             &\le \frac{1}{n}\sum\limits_{k=1}^{n}{|a_k - a|} \\
             &= \frac{1}{n}\sum\limits_{k=1}^{N}{|a_k - a|} + \frac{1}{n}\sum\limits_{k=N+1}^{n}{|a_k - a|} \\
             &< \frac{1}{n}\sum\limits_{k=1}^{N}{|a_k - a|} + \frac{n - N}{n} \cdot \frac{\epsilon}{2} \\
             &= \frac{1}{n}\sum\limits_{k=1}^{N}{|a_k - a|} + \left(1 - \frac{N}{n}\right) \cdot \frac{\epsilon}{2}
        \end{align*}

        Furthermore, $0 < \frac{N}{n} < 1$ and hence 
        $\left(1 - \frac{N}{n}\right) < 1$. Since 
        $\sum\limits_{k=1}^{N}{|a_k - a|}$ is a finite series made up of
        positive terms, we pick
        $n > \max{\{N, \frac{2}{\epsilon} \cdot \sum\limits_{k=1}^{N}{|a_k - a|}\}}$.
        Thus we have for such an $n$ that:

        \begin{align*}
            \frac{1}{n}\sum\limits_{k=1}^{N}{|a_k - a|} + \left(1 - \frac{N}{n}\right) \cdot \frac{\epsilon}{2}
              &< \frac{\epsilon}{2} + \left(1 - \frac{N}{n}\right) \cdot \frac{\epsilon}{2} \\
              &\le \frac{\epsilon}{2} + \frac{\epsilon}{2} \\
              &= \epsilon.
        \end{align*}

        By the $\epsilon$-definition of a limit,
        $\lim_{n \rightarrow \infty}{\sigma_n} = a$.
        \pagebreak

        To prove that the converse does not hold, let $\{a_n\}$ be the
        sequence defined by:

        \begin{align*}
            a_n = (-1)^{n+1}.
        \end{align*}
        
        Then $\lim_{n \rightarrow \infty}{a_n}$ does not exist since the odd
        terms are 1 and the even terms are -1. The $n^{th}$ term of
        $\sigma_n$ is thus given by:

        \begin{align*}
            \sigma_1 &= \frac{1}{1} = 1 \\
            \sigma_2 &= \frac{1 - 1}{2} = 0 \\
            \sigma_3 &= \frac{1 - 1 + 1}{3} = 1/3 \\
            \sigma_4 &= \frac{1 - 1 + 1 - 1}{4} = 0 \\
            \sigma_5 &= \frac{1 - 1 + 1 - 1 + 1}{5} = 1/5 \\
                     &\vdots \\
            \sigma_n &= \frac{1 - (-1)^n}{2n} \\
        \end{align*}

        Since $\lim_{n \rightarrow \infty}{\sigma_n = \frac{1 - (-1)^n}{2n}} = 0$,
        we have that
        $\lim_{n \rightarrow \infty}{\sigma_n} \neq \lim_{n \rightarrow \infty}{a_n}$.
        \\\\
    \end{proof}
    \pagebreak

b.  For a real sequence $\{a_n\}$, define $d_n \coloneqq a_{n+1} - a_n$ for
    $n \ge 1$. If $\lim_{n \rightarrow \infty}{nd_n} = 0$ and the sequence
    $\{\sigma_n\}$ defined in part (a) converges, prove that the sequence
    $\{a_n\}$ converges and that
    $\lim_{n \rightarrow \infty}{a_n} = \lim_{n \rightarrow \infty}{\sigma_n}$.
    (Hint: Show that $\frac{1}{n}\sum\limits_{k=1}^{n-1}{kd_k} = a_n - \sigma_n$
     for $n > 1$).

    \begin{proof}\ \\\\

        To demonstrate the provided hint, observe that:

        \renewcommand*{\thefootnote}{\fnsymbol{footnote}}
        \begin{align*}
            \sum\limits_{k=1}^{n-1}{kd_k} &= 1d_1 + 2d_2 + 3d_3 + \cdots + (k - 1)d_{k-1} \\
                                          &= 1(a_2 - a_1) 
                                           + 2(a_3 - a_2)
                                           + 3(a_4 - a_3)
                                           + \cdots
                                           + (n - 2)(a_{n-1} - a_{n-2})\footnotemark[2]
                                           + (n - 1)(a_n - a_{n-1}) \\
                                          &= -a_1 
                                             + (1 - 2)a_2 
                                             + (2 - 3)a_3
                                             +  \cdots
                                             +  \left[(n - 2) - (n - 1)\right]a_{n-1}
                                             + (n-1)a_{n} \\
                                          &= -a_1 
                                             - a_2
                                             - a_3 
                                             - \cdots
                                             - a_{n-1}
                                             - a_n + na_{n} \\
                                          &= na_n - n\sum\limits_{k=1}^{n}{\frac{a_1 + a_2 + \cdots + a_n}{n}} \\
                                          &= n(a_n - \sigma_n).
        \end{align*}

        Hence $\frac{1}{n}\sum\limits_{k=1}^{n-1}{kd_k} = a_n - \sigma_n$ and
        in particular, $\frac{1}{n}\sum\limits_{k=1}^{n-1}{kd_k} =  - d_n + \frac{1}{n}\sum\limits_{k=1}^{n}{kd_k}$.
        \\\\
        \footnotetext[2]{
            Observe that the $-a_{n-2}(n-2)$ term gets grouped with a
            corresponding $(n-3)a_{n-2}$ term from the previous summand in the
            series. Hence we omit this value in the next line, as it is
            understood to be included in the implicit summation term.
        }

        \pagebreak
        Because
        $\left\{\frac{1}{n}\sum\limits_{k=1}^{n}{kd_k}\right\}$ converges to
        zero as the CesÃ ro sum of $\{kd_k\}$ by part (a) and because $\{d_k\}$
        also converges to zero\footnotemark[3], for any fixed $\epsilon > 0$
        there exist corresponding $N_1, N_2 \in \mathbb{N}$ such that
        $\left|\frac{1}{n}\sum\limits_{k=1}^{n}{kd_k}\right| < \frac{\epsilon}{4}$
        and $|d_n| < \frac{\epsilon}{4}$ whenever $n > \max{\{N_1, N_2\}}$. Let
        $a$ be the limit to which $\{\sigma_n\}$ converges. Then there exists
        an $N_3$ such that $|(\sigma_n - a)| < \frac{\epsilon}{2}$ whenever
        $n > N_3$. Defining $N \coloneqq \max{\{N_1, N_2, N_3}\}$ we have for
        $n > N$ that:

        \footnotetext[3] {
            Since $|d_k| \le k\left|d_k\right|$ and $\{kd_k\}$ converges to
            zero, $\{d_k\}$ itself must also converge to zero.
        }

        \begin{align*}
            |a_n - a| &= |a_n - a| - \frac{\epsilon}{2} + \frac{\epsilon}{2} \\
                      &\le \left| |a_n - a| - \frac{\epsilon}{2}\right| + \frac{\epsilon}{2}  \\
                      &\le \Big| |a_n - a | - |\sigma_n - a| \Big| + \frac{\epsilon}{2}  \\
                      &\le |(a_n - a ) - (\sigma_n - a)| + \frac{\epsilon}{2} \\
                      &= |a_n - \sigma_n| + \frac{\epsilon}{2} \\
                      &= \left|\frac{1}{n}\sum\limits_{k=1}^{n-1}{kd_k}\right| + \frac{\epsilon}{2} \\
                      &= \left| -d_n + \frac{1}{n}\sum\limits_{k=1}^{n}{kd_k} \right| + \frac{\epsilon}{2} \\
                      &\le |-d_n| + \left|\frac{1}{n}\sum\limits_{k=1}^{n}{kd_k}\right| + \frac{\epsilon}{2} \\
                      &< \frac{\epsilon}{4} + \frac{\epsilon}{4} + \frac{\epsilon}{2} \\
                      &= \epsilon. \\
        \end{align*}

        Since $|a_n - a| < \epsilon$ for any arbitrary $\epsilon > 0$, we have
        that  $\lim_{n \rightarrow \infty}{a_n} = a = \lim_{n \rightarrow \infty}{\sigma_n}$.
        \\\\
        \renewcommand*{\thefootnote}{\arabic{footnote}}

    \end{proof}