a.  Use the Mean Value Theorem to show that
    $\frac{x}{1 + x} \le \ln{\left(1 + x\right)} \le x$ for $x \ge 0$. Evaluate at
    $x = \frac{1}{n}$ to show that:

    \begin{align*}
        \frac{1}{n+1} \le \ln{\left(1 + \frac{1}{n}\right)} \le \frac{1}{n}
    \end{align*}

    \begin{proof}\ \\\\
        Observe that $f(x) = \ln{(1+x)}$ is continuous on $[0, x]$ and
        differentiable on $(0, x)$. Hence by the Mean Value Theorem, there
        exists some $c \in (0, x)$ such that:
    
        \begin{align*}
            f'(c) &= \frac{\ln(1+x) - \ln(1+0)}{x-0} \\
            \frac{1}{1+c} &= \frac{\ln(1+x)}{x}
        \end{align*}

        Since $0 < \frac{1}{1+c} \le 1$ for all $c \in [0, \infty)$, we have
        that $\frac{\ln{(1+x)}}{x} \le 1$ and hence $\ln{(1+x)} \le x$, which
        satisfies the right-most inequality.

        To prove the left inequality, we define
        $h(x) \coloneqq \frac{x}{1+x} - \ln{(1+x)}, x \in [0, \infty)$. Then
        $h(x)$ is continuous and differentiable on its domain and hence by the
        Mean Value Theorem there exists some $c \in (0, x)$ such that:

        \begin{align*}
            f'(c) &= \frac{\frac{x}{1+x} - \ln(1+x) - \left(\frac{0}{1+0} - \ln(1+0)\right)}{x-0} \\
            \frac{1}{(1+c)^2} - \frac{1}{1+c} &= \frac{1}{x} \cdot \left(\frac{x}{1+x} - \ln(1+x)\right) \\
            x\left(\frac{1}{(1+c)^2} - \frac{1}{1+c}\right) &= \frac{x}{1+x} - \ln(1+x)
        \end{align*}

        Observe that $(1+c)^2 > 1+c, c \in (0, \infty)$ and hence 
        $\frac{1}{(1+c)^2} - \frac{1}{1+c} < 0$. Since $x \ge 0$, we see that
        $x\left(\frac{1}{(1+c)^2} - \frac{1}{1+c}\right) \le 0$. Thus,
        $\frac{x}{1+x} - \ln(1+x) \le 0$ and so $\frac{x}{1+x} \le \ln(1+x)$,
        which satisfies the left-most inequality.

        Lastly, since $\frac{\frac{1}{n}}{1 + \frac{1}{n}} = \frac{n}{n(n+1)} = \frac{1}{n+1}$,
        we have for $x = \frac{1}{n}$ that:

        \begin{align*}
            \frac{1}{n+1} \le \ln{\left(1 + \frac{1}{n}\right)} \le \frac{1}{n}
        \end{align*}

        as desired.
    \end{proof}
    \pagebreak

b.  Define $\gamma_n \coloneqq \left(1 + \frac{1}{2} + \frac{1}{3} + \cdots + \frac{1}{n} \right) - \ln{n}.$
    Use part (a) to show that $\gamma_n \ge 0$ and that $\{\gamma_n\}$ is a
    decreasing sequence.

    \begin{proof}\ \\\\

        We first show that $\{\gamma_n\}$ is decreasing. Observe that:

        \begin{align*}
            \gamma_{n+1} - \gamma_n &= \sum\limits_{k=1}^{n+1}{\frac{1}{k}} - \ln{(n+1)} - \left(\sum\limits_{k=1}^{n}{\frac{1}{k}} - \ln{n}\right) \\
                                    &= \frac{1}{1+n} - \left[\ln{(n+1)} - \ln{n}\right] \\
                                    &= \frac{1}{1+n} - \ln{\frac{n+1}{n}} \\
                                    &= \frac{1}{1+n} - \ln{\left(1 + \frac{1}{n}\right)} \\
        \end{align*}

        By the left-most inequality from (a) we have that
        $\gamma_{n+1} - \gamma_n \le 0$ and hence $\{\gamma_n\}$ is decreasing.
        \\\\

        To show that $\gamma_n \ge 0$, recall from (a) that for each
        $k \in \mathbb{N}$:

        \begin{align*}
            \frac{1}{k} &\ge \ln{\frac{k + 1}{k}} 
        \end{align*}

        Summing each side from 1 to $n$ yields:

        \begin{align*}
             \sum\limits_{k=1}^{n}{\frac{1}{k}} &\ge \sum\limits_{k=1}^{n}{\ln{\frac{k + 1}{k}}} \\
                                                &= \sum\limits_{k=1}^{n}{\ln{(k + 1) - \ln{k}}}  \\
                                                &= \left[\ln{(n+1)}  - \ln{n}\right] + \left[\ln{n} - \ln{(n-1)}\right] + \cdots - \ln{1} \\
                                                &= \ln{(n+1)} \\
                                                &\ge \ln{n}.
        \end{align*}

        Hence $\gamma_n = \sum\limits_{k=1}^{n}{\frac{1}{k}} - \ln{n} \ge 0$.

    \end{proof}

    \pagebreak

c.  Show that $\{\gamma_n\}$ converges. (Extra credit: Prove that $\gamma > 0$).

    \begin{proof}\renewcommand{\qedsymbol}{}\ \\\\
        Observe that $\gamma_1 = \frac{1}{1} - \ln{1} = 1$. By part (b),
        $\{\gamma_n\}$ is decreasing and bounded below by 0. Hence 
        $\{\gamma_n\}$ is bounded and monotonically decreasing in $\mathbb{R}$,
        and therefore converges.
        \\

        TODO: Show that $\gamma > 0$. To show that $\gamma > 0$, we should find a
        non-zero lower bound for $\{\gamma_n\}$.

        \begin{align*}
        \end{align*}
        \\\\
    \end{proof}