a.  Let $\{a_n\}$ be a sequence of real numbers such that 
    $|a_{n+1} - a_n| < 3^{-n}$ for all $n \in \mathbb{N}$. Prove that $\{a_n\}$
    is a convergent sequence.  \\

    \begin{proof}\ \\\\
        Observe that $\sum\limits_{k=0}^{\infty}{\frac{1}{3^{n}}} = \sum\limits_{k=0}^{\infty}{\left(\frac{1}{3}\right)^n}$
        converges as a geometric series, and hence the sequence of partial sums 
        $s_n \coloneqq \sum\limits_{k=1}^{n}{\frac{1}{3^{n}}}$ is Cauchy
        sequence.  Hence for any fixed $\epsilon > 0$, there exists some $N > 0$
        such that for all $m > n > N$, $|s_m - s_n| < \epsilon$. For such $m$ 
        and $n$, we have:
    
        \begin{align*}
            |a_m - a_n| &= |a_m - a_{m-1} + a_{m-1} - a_{m-2} + a_{m-2} + \cdots - a_n | \\
                        &\le |a_m - a_{m-1}| + |a_{m-1} - a_{m-2}| + \cdots + |a_{n+1} - a_n | \\
                        &\le \sum\limits_{k=n}^m{3^{-k}} \\ 
                        &= |s_m - s_n| \\
                        &< \epsilon.
        \end{align*}
    
        Hence $\{a_n\}$ is Cauchy and since $\mathbb{R}$ is complete, $\{a_n\}$
        converges to a value also in $\mathbb{R}$ and $\{a_n\}$ is therefore a
        convergent sequence.
    \end{proof}
    \ \\\\

b.  Let $\{a_n\}$ and $\{b_n\}$ be real sequences such that
    $|a_n - b_n| \le 1/n$ for all $n \in \mathbb{N}$, and $a_n \rightarrow L$.
    Prove that $b_n \rightarrow L$. \\

    \begin{proof}\ \\\\
        Since $\lim_{n \rightarrow \infty}{\frac{1}{n}} = 0$, for any fixed 
        $\epsilon > 0$ there exists $N_1$ such that when $n > N_1$,
        $|\frac{1}{n} - 0| = \frac{1}{n} < \frac{\epsilon}{2}$. Similarly,
        since $\lim_{n \rightarrow \infty}{\{a_n\}} = L$, there exists $N_2$
        such that when $n > N_2$, $|a_n - L| < \frac{\epsilon}{2}$. \\\\
        
        Let $N \coloneqq \max{\{N_1, N_2\}}$. Then for $n > N$ we have:


        \begin{align*}
            |a_n - b_n| &= |b_n - a_n| \\
                        &= |(b_n - L) - (a_n - L)| \\
                        &\ge \bigl| |b_n - L| - |a_n - L|\bigl| \\
        \end{align*}

        Distributing the absolute value yields:


        \begin{align*}
            |a_n - b_n| &\ge |b_n - L| - |a_n - L| \ge -|a_n - b_n|
        \end{align*}

        Adding $|a_n - L|$ to each term and rearranging the left inequality 
        yields:

        \begin{align*}
            |b_n - L| &\le |a_n - b_n| + |a_n - L| \\
                      &< \frac{\epsilon}{2} + \frac{\epsilon}{2} \\
                      &= \epsilon.
        \end{align*}

        Hence by the $\epsilon$-definition of a limit, we have that 
        $\lim_{n \rightarrow \infty}{b_n} = L$.

    \end{proof}