The 3-step Adams-Bashforth method.

\begin{solution}\ \\\\
    Recall that the 3-step Adams-Moulton method may be written as follows:

    $$
    -U^{n+2} + U^{n+3} = k \left(\frac{1}{24} f(U^n) - \frac{5}{24} f(U^{n+1}) + \frac{19}{24} f(U^{n+2}) + \frac{9}{24} f(U^{n+3}) \right)
    $$

    The characteristic polynomials $\phi(\zeta)$ and $\sigma(\zeta)$ may therefore be written:

    \begin{align*}
        \phi(\zeta)   &= -\zeta^2 + \zeta^3 \\
        \sigma(\zeta) &= \frac{1}{24} - \frac{5}{24} \zeta + \frac{19}{24} \zeta^2  + \frac{9}{24} \zeta^3.
    \end{align*}

    Moreover, we have 
    
    $$
    \sum\limits_{j=0}^{r}{\alpha_j = \alpha_2 + \alpha_3} = -1 + 1 = 0
    $$

    and 
    
    $$
    \sum\limits_{j=0}^{r}{j \alpha_j - \beta_j} = 2 \cdot (-1) + 3 \cdot 1 - \left(\frac{1}{24} - \frac{5}{24} + \frac{19}{24} + \frac{9}{24} \right) = 0
    $$

    and so (5.48) holds.

    \ \\
\end{solution}