Let 

$$
R(z) = \frac{1 + z/2}{1 - z/2}.
$$

Show that $R(z) = e^z + \mathcal{O}(z^3)$ and conclude that the one-step error of the trapezoidal method on this problem
is $\mathcal{O}(k^3)$.

\begin{solution}\ \\\\
    Let $k < \frac{1}{\lambda}$. Then we have

    $$
    \frac{1}{1 - z/2} = \sum\limits_{n=0}^{\infty}{\left(\frac{z}{2}\right)^n}
    $$

    as a geometric series. We multiply this series by $(1 + z/2)$ to find:

    \begin{align*}
    \frac{1 + z/2}{1 - z/2} &= \left(1 + \frac{z}{2}\right) \sum\limits_{n=0}^{\infty}{\left(\frac{z}{2}\right)^n} \\
                            &= \left(1 + \frac{z}{2}\right) 
                             + \left(1 + \frac{z}{2}\right) \frac{z}{2} 
                             + \left(1 + \frac{z}{2}\right) \left(\frac{z}{2} \right)^2 
                             + \left(1 + \frac{z}{2}\right) \sum\limits_{n=3}^{\infty}{\left(\frac{z}{2}\right)^n} \\
                            &= 1 + z + \frac{z^2}{2} + \frac{z^3}{4}  
                             + \left(1 + \frac{z}{2}\right) \sum\limits_{n=3}^{\infty}{\left(\frac{z}{2}\right)^n} \\
                            &= 1 + z + \frac{z^2}{2!} + \left( \frac{2z^3}{24} + \frac{x^3}{3!} \right)
                             + \left(1 + \frac{z}{2}\right) \sum\limits_{n=3}^{\infty}{\left(\frac{z}{2}\right)^n} \\
                            &= e^z + \frac{2z^3}{24} 
                             + \sum\limits_{n=3}^{\infty}{\left(1 + \frac{z}{2}\right) \left(\frac{z}{2}\right)^n - \frac{z^{n+1}}{(n+1)!}} \\
                            &= e^z + \mathcal{O}(z^3).
    \end{align*}

    Since $z = \lambda k$, we have:

    \begin{align*}
    U^{n+1} &= \left( \frac{1 + z/2}{1 - z/2} \right) U^n \\
            &= \left[e^{\lambda k} + \mathcal{O}\left( k^3 \lambda^3 \right)\right] U^n \\
            &= \mathcal{O}\left( k^3 \right) U^n.
    \end{align*}

    Hence the one-step error of the trapezoidal method on this problem is $\mathcal{O}(k^3)$, as desired.
    \ \\
\end{solution}