(\#3 in 2.2) Prove or disprove the following:
For $B\subseteq Y$ and $f:X\to Y$, $f^{-1}(Y\backslash B)=X\backslash f^{-1}(B)$. 

\ \\
\emph{Claim.} For $B\subseteq Y$ and $f:X\to Y$, $f^{-1}(Y\backslash B)$ is 
equal to $X\backslash f^{-1}(B)$.

\begin{proof}\ \\\\
    Observe that by definition, $f^{-1}(Y \backslash B) = \left\{x \in X | f(x) \in Y \backslash B\right\}$.
    Furthermore, $X \backslash f^{-1}(B)$ is the set of all elements in $X$ whose image is not in $B$, i.e., it
    is the set of all elements whose image is in $Y \backslash B$ (since the co-domain $Y$ by definition contains the
    image of $X$). Hence $X \backslash f^{-1}(B) = \left\{x \in X | f(x) \in Y \backslash B\right\}$, and so
    $f^{-1}(Y\backslash B) = X\backslash f^{-1}(B)$.
    \ \\
\end{proof}