\textbf{Griva, Nash, Sofer 2.3.2}

Let $S_1 = \left\{ x \mid 1 - x_1 - x_2 \ge 0, x_1 \ge 0 \right\}$ and 
$S_2 = \left\{ x \mid x_1 - x_2 \ge 0, 1 - x_1 \ge 0 \right\}$, and let $S = S_1 \cup S_2$.
Prove that $S_1$ and $S_2$ are both convex sets but $S$ is not a convex set (and conclude
that the union of convex sets is not necessarily convex).

\begin{solution}
  Let $c, b \in \mathbb{R}^n$ and let $S = \left\{ x \mid c^T x \le b \right\}$ represent an arbitrary linear constraint
  in $\mathbb{R}^n$. We first show that $S$ is convex, and subsequently apply this result to $S_1$ and $S_2$. Let $x$ 
  and $y$ be arbitrary points in $S$. Then $c^T x \le b$ and $c^T y \le b$, and we wish to show that 
  $\alpha x + (1 - \alpha) y \in S$ for any $\alpha \in [0, 1]$. We multiply $\alpha x + (1 - \alpha) y$ by $c^T$ to find 
  (by linearity and the observation that both $\alpha$ and $1 - \alpha$ are non-negative):

  \begin{align*}
    c^T \left(\alpha x + (1 - \alpha) y \right) &= c^T \alpha x + c^T (1 - \alpha) y \\
                                                &= \alpha c^T x + (1 - \alpha) c^T y \\
                                                &\le \alpha b + (1 - \alpha) b \\
                                                &= \alpha b + b - \alpha b \\
                                                &= b \\
  \end{align*}

  Hence $\alpha x + (1 - \alpha) y \in S$ and so $S$ is convex, as desired. To show $S_1$ and $S_2$ are convex, we restrict
  our attention to $\mathbb{R}^2$ and observe that we may write

  $$
  S_1 = \{x \mid x_1 + x_2 \le 1\} \cap \{ x \mid -x_1 \le 0 \}.
  $$

  Letting $c = (1, 1)\;, b = 1$ for the first linear constraint and $c = (-1, 0)\;, b = 0$ for the second and applying
  our result from 2.3.1, we have that $S_1$ is convex. We similarly write

  $$
  S_2 = \{x \mid -x_1 + x_2 \le 0\} \cap \{ x \mid x_1 \le 1 \}
  $$

  and let $c = (-1, 1)\;, b = 0$ for the first linear inequality and $c = (1, 0)\;, b = 1$ for the second to find that
  $S_2$ is also convex.

  Lastly, to show that $S_1 \cup S_2$ is \textit{not} convex, we consider the points $x = (0, 1)^T \in S_1$ and 
  $y = (1, 1)^T \in S_2$ and let $\alpha = \frac{1}{2}$ to find:

  $$
  \frac{1}{2}x + \left(1 - \frac{1}{2}\right)y = \left(0, \frac{1}{2}\right)^T + \left(\frac{1}{2}, \frac{1}{2}\right)^T
                                               = \left(\frac{1}{2}, 1\right)^T \notin S_1 \cup S_2,
  $$

  since $x_1 + x_2 = \frac{1}{2} + 1 \nleq 1$ and $-x_1 + x_2 = -\frac{1}{2} + 1 = \frac{1}{2} \nleq 0$.

  \ \\
\end{solution}