Prove that if $\tilde{k}^2 = 1 - k^2$ and $0 < \tilde{k} < 1$, then

$$
K'(k) = K(\tilde{k}).
$$

\newcommand{\kt}{\tilde{k}}

\textit{Hint:} Change variables $x = \left(1 - \tilde{k}^2 y^2\right)^{-\frac{1}{2}}$ in the integral which defines $K'(k)$.

\begin{solution}
  We begin by changing variables as in the hint so that

  $$
  dx = -\frac{1}{2}\left(1 - \kt^2 y^2 \right)^{-\frac{3}{2}}\left(-2 \kt^2 y\right) dy 
     = \frac{\kt^2 y}{\left(1 - \kt^2 y^2\right)^{\frac{3}{2}}} dy.
  $$

  For the limits of integration $a$ and $b$ for $K'(k)$ under the above coordinate transformation, we have

  $$
  a = 1 
    = \left(1 - \kt^2 y^2\right)^{-\frac{1}{2}} 
      \implies 1 = 1 - \kt^2 y^2 
      \implies y = 0,
  $$

  since $0 < \kt < 1$. Moreover, we have

  $$
  b = \frac{1}{k} 
    = \left(1 - \kt^2 y^2\right)^{-\frac{1}{2}} 
      \implies 1 - \kt^2 y^2 = k^2 
      \implies y = \sqrt{\frac{1 - k^2}{\kt^2}} = 1,
  $$

  since $1 - k^2 = \kt^2$ and $0 < \kt < 1$. Our integrand for $K'(k)$ then becomes:

  \begin{align*}
    \frac{1}{\sqrt{\left(x^2 - 1\right)\left(1 - k^2 x^2\right)}} \, dx
      &= \frac{1}{\left[\left(\frac{1}{1 - \kt^2 y^2} - 1 \right) \left(1 - \frac{k^2}{1 - \kt^2 y^2} \right)\right]^{\frac{1}{2}}}
         \frac{\kt^2 y}{\left(1 - \kt^2 y^2\right)^{\frac{3}{2}}} \, dy \\
      &= \frac{1}{\left[\left(\frac{\kt^2 y^2}{1 - \kt^2 y^2}\right) \left(\frac{1 - \kt^2 y^2 - k^2}{1 - \kt^2 y^2} \right)\right]^{\frac{1}{2}}}
         \frac{\kt^2 y}{\left(1 - \kt^2 y^2\right)^{\frac{3}{2}}} \, dy \\
      &= \frac{1}{\left[\left(\frac{\kt^2 y^2}{1 - \kt^2 y^2}\right) \left(\frac{\kt^2 - \kt^2 y^2}{1 - \kt^2 y^2} \right)\right]^{\frac{1}{2}}}
         \frac{\kt^2 y}{\left(1 - \kt^2 y^2\right)^{\frac{3}{2}}} \, dy \\
      &= \frac{\kt^2 y}{\left[\kt^4 y^2 (1 - y^2)(1 - \kt^2 y^2) \right]^{\frac{1}{2}}} \, dy \\
      &= \frac{1}{\left[(1 - y^2)(1 - \kt^2 y^2) \right]^{\frac{1}{2}}} \, dy \\
  \end{align*}

  so that with our transformed limits of integration, we have 

  \begin{align*}
    K'(k) &= \int_1^{\frac{1}{k}} \frac{1}{\sqrt{\left(x^2 - 1\right)\left(1 - k^2 x^2\right)}} \, dx \\
          &= \int_0^1 \left[(1 - y^2)(1 - \kt^2 y^2) \right]^{-\frac{1}{2}} \, dy \\
          &= K(\kt),
  \end{align*}

  as was to be shown.
  \ \\
\end{solution}