Prove that if $\tilde{k}^2 = 1 - k^2$ and $0 < \tilde{k} < 1$, then

$$
K(k) = \frac{2}{1 + \tilde{k}} K\left(\frac{1 - \tilde{k}}{1 + \tilde{k}} \right)
$$

\textit{Hint:} Change variables by letting $x = \frac{2t}{1 + \tilde{k} + \left(1 - \tilde{k}\right) t^2}$.

\begin{solution}
  We begin by showing that the above transformation preserves the limits of integration. We first note that since 
  $0 < \kt < 1$, the quantities $1 + \kt$ and $1 - \kt$ are both positive. From this, we observe that

  $$
  a = 0
    = \frac{2t}{\left(1 + \kt\right) + \left(1 - \kt\right) t^2}
      \implies t = 0.
  $$

  For the other limit of integration, we observe that

  $$
  b = 1 
    = \frac{2t}{\left(1 + \kt\right) + \left(1 - \kt\right) t^2}
      \implies (1 - \kt)t^2 - 2t + (1 + \kt) = 0
  $$

  where an application of the quadratic formula yields the roots $t = 1$ and $t = \frac{1 - \kt}{1 + \kt}$. We choose
  the former root since the latter is greater than 1. 
 
  as was to be shown. We now define $\alpha \coloneqq \frac{1 - \kt}{1 + \kt} > 0$ so that 
 
  $$
    x = \frac{1}{1 + \kt}\frac{2t}{1 + \alpha t^2} \quad \text{and} \quad x^2 = \frac{1}{(1 + \kt)^2}\frac{4t^2}{(1 + \alpha t^2)^2}.
  $$

  and 

  $$
  dx = \frac{1}{1 + \kt} \frac{2 - 2 \alpha t^2}{(1 + \alpha t^2)^2} \, dt 
     = \frac{2}{1 + \kt} \frac{1 - \alpha t^2}{(1 + \alpha t^2)^2} \, dt.
  $$

  Before proceeding with the proof, we show two useful identities. First, we have

  \begin{equation} \label{eq:5b-identity-the-first}
    1 + \alpha^2 = \frac{\left(1 + \kt\right)^2 + \left(1 - \kt\right)^2}{\left(1 + \kt\right)^2}
                 = \frac{2\left(1 + \kt^2\right)}{\left(1 + \kt\right)^2},
  \end{equation}

  and secondly 

  $$
    k^2 = 1 - \kt^2 = \left(1 + \kt\right)\left(1 - \kt\right)
  $$

  so that after dividing both sides by $\left(1 + \kt\right)^2$, we obtain

  \begin{equation} \label{eq:5b-identity-the-second}
    \frac{k^2}{\left(1 + \kt\right)^2} = \frac{1 - \kt}{1 + \kt} = \alpha.
  \end{equation}

  We now substitute our change of variables into $K(k)$ to obtain

  \begin{align*}
    K(k) &= \int_0^1 \frac{dx}{\left[(1 - x^2) (1 - k^2 x^2) \right]^{\frac{1}{2}}} \\
         &= \frac{2}{1 + \kt} \int_0^1 \frac{1 - \alpha t^2}{\left(1 + \alpha t^2\right)^2}
            \left[
              \left(
                1 - \frac{4t^2}{\left(1 + \kt \right)^2 \left(1 + \alpha t^2 \right)^2}
              \right)
              \left(
                1 - \frac{4k^2t^2}{\left(1 + \kt \right)^2 \left(1 + \alpha t^2 \right)^2}
              \right)
            \right]^{-\frac{1}{2}} \, dt \\
         &= \frac{2}{1 + \kt} \int_0^1 (1 - \alpha t^2)
            \left[
              \left(
                \left(1 + \alpha t^2\right)^2 - \frac{4t^2}{\left(1 + \kt \right)^2}
              \right)
              \left(
                \left(1 + \alpha t^2\right)^2 - \frac{4k^2t^2}{\left(1 + \kt \right)^2}
              \right)
            \right]^{-\frac{1}{2}} \, dt
  \end{align*}

  For the first term in square brackets, we apply the identity in \eqref{eq:5b-identity-the-first} to obtain

  \begin{align*}
    \left(1 + \alpha t^2\right)^2 - \frac{4t^2}{\left(1 + \kt \right)^2} 
      &= 1 + 2 \alpha t^2 + \alpha^2 t^4 - \frac{4t^2}{\left(1 + \kt \right)^2} \\ 
      &= 1 + \frac{2 (1 - \kt)(1 + \kt) t^2 + (1 - \kt)^2 t^4 - 4t^2}{\left(1 + \kt \right)^2} \\ 
      &= 1 + \frac{2 (1 - \kt^2) t^2 + (1 - \kt)^2 t^4 - 4t^2}{\left(1 + \kt \right)^2} \\ 
      &= 1 + \frac{t^2(2 - 2\kt^2 - 4) + (1 - \kt)^2 t^4}{\left(1 + \kt \right)^2} \\ 
      &= 1 + \alpha^2 t^4 - \frac{2 t^2(1 + \kt^2)}{\left(1 + \kt \right)^2} \\ 
      &= 1 + \alpha^2 t^4 - (1 + \alpha^2) t^2 \\
      &= (1 - t^2)(1 - \alpha^2 t^2)
  \end{align*}

  Similarly, we apply \eqref{eq:5b-identity-the-second} to the second term in square brackets to obtain

  $$
  \left(1 + \alpha t^2\right)^2 - \frac{4k^2t^2}{\left(1 + \kt \right)^2} 
    = (1 + 2 \alpha t^2 + \alpha^2 t^4) - 4 \alpha t^2
    = \left(1 - \alpha t^2\right)^2,
  $$

  \pagebreak
  Substituting these two results back into our current expression for $K(k)$ yields

  \begin{align*}
    K(k) &= \frac{2}{1 + \kt} \int_0^1 (1 - \alpha t^2)
            \left[
              \left(
                \left(1 + \alpha t^2\right)^2 - \frac{4t^2}{\left(1 + \kt \right)^2}
              \right)
              \left(
                \left(1 + \alpha t^2\right)^2 - \frac{4k^2t^2}{\left(1 + \kt \right)^2}
              \right)
            \right]^{-\frac{1}{2}} \, dt \\
         &= \frac{2}{1 + \kt} \int_0^1 (1 - \alpha t^2)
            \left[
              (1 - t^2)(1 - \alpha^2 t^2) \left(1 + \alpha t^2\right)^2 
            \right]^{-\frac{1}{2}} \, dt \\
         &= \frac{2}{1 + \kt} \int_0^1 
            \left[
              (1 - t^2)(1 - \alpha^2 t^2)
            \right]^{-\frac{1}{2}} \, dt \\
          &= \frac{2}{1 + \kt} K(\alpha),
  \end{align*}

  as desired.
  \ \\
\end{solution}