Show that for $0 < k < 1$, one has

$$
K(k) = \frac{\pi}{2} F \left(\frac{1}{2}, \frac{1}{2}, 1; \; k^2 \right),
$$

where $F$ is the hypergeometric series given by

$$
F(\alpha, \beta, \gamma; \; z) = \frac{\Gamma(\gamma)}{\Gamma(\beta)\Gamma(\gamma - \beta)} 
                                 \int_0^1 t^{\beta - 1} (1 - t)^{\gamma - \beta - 1} (1 - zt)^{-\alpha} \, dt
$$

with $\alpha, \beta > 0$, $\gamma > \beta$, and $|z| < 1$. 

\ \\
\textit{Hint:} This follows from the integral representation for $F$ given in Exercise 6.9 of \textit{Stein, Shakarchi}.

\begin{solution}
  Upon substituting $\alpha = \beta = \frac{1}{2}$, $\gamma = 1$, and $z = k^2$ into the integral representation for $F$ 
  given above and noting that $\Gamma\left(\frac{1}{2}\right) = \sqrt{\pi}$, we have:

  \begin{align*}
  \frac{\pi}{2} F \left(\frac{1}{2}, \frac{1}{2}, 1; \; k^2 \right) 
    &= \frac{\pi}{2} \frac{\Gamma(1)}{\Gamma\left(\frac{1}{2}\right)\Gamma\left(\frac{1}{2}\right)} 
       \int_0^1 t^{-\frac{1}{2}} (1 - t)^{-\frac{1}{2}} (1 - k^2 t)^{-\frac{1}{2}} \, dt \\
    &= \frac{1}{2} \int_0^1 \frac{1}{t^{-\frac{1}{2}} \left[(1 - t)(1 - k^2 t)\right]^{\frac{1}{2}}} \, dt
  \end{align*}

  We now change variables by letting $t = x^2$ so that $dt = 2x \, dx$ and our integrands remain unchanged. Our 
  integral therefore becomes:

  \begin{align*}
  \frac{\pi}{2} F \left(\frac{1}{2}, \frac{1}{2}, 1; \; k^2 \right) 
    &= \frac{1}{2} \int_0^1 \frac{1}{t^{\frac{1}{2}} \left[(1 - t)(1 - k^2 t)\right]^{\frac{1}{2}}} \, dt \\
    &= \frac{1}{2} \int_0^1 \frac{2 x}{x \left[(1 - x^2)(1 - k^2 x^2)\right]^{\frac{1}{2}}} \, dx \\
    &= \int_0^1 \frac{1}{\left[(1 - x^2)(1 - k^2 x^2)\right]^{\frac{1}{2}}} \, dx \\
    &= K(k),
  \end{align*}

  as was to be shown.
  \ \\
\end{solution}