\textbf{Lang 8.4.2}

Let $0 \le r < R$ and define

$$
P_{R, r}(\theta) = \frac{1}{2 \pi} \frac{R^2 - r^2}{R^2 - 2 R r \cos{\theta} + r^2}.
$$

Prove that the following inequality holds:

$$
\frac{R - r}{R + r} \le 2 \pi P_{R, r}(\theta - \phi) \le \frac{R + r}{R - r}.
$$

\begin{solution}
  For notational simplicity, we define $\alpha = \theta - \phi$. We begin with the observation that 

  $$
  -1 \le \cos{\alpha} \le 1.
  $$

  Since $0 \le r < R$, we obtain the following inequality after multiplying by $-2 R r$ and adding $R^2 + r^2$:

  $$
  (R + r)^2 = R^2 + 2 R r + r^2 
            \ge R^2 - 2 R r \cos{\alpha} + r^2 
            \ge R^2 - 2 R r + r^2 
            = (R - r)^2 > 0.
  $$

  From this inequality (along with the observation that $R - r > 0$ since $R > r$), we conclude that

  $$
  \frac{R - r}{R + r} = \frac{R^2 - r^2}{(R + r)^2} 
                      \le 2 \pi \left(\frac{1}{2 \pi} \frac{R^2 - r^2}{R^2 - 2 R r \cos{\alpha} + r^2} \right)
                      \le \frac{R^2 - r^2}{(R - r)^2} 
                      = \frac{R + r}{R - r}
  $$

  as desired.
  \ \\
\end{solution}
